main.v
@@ -6,18 +6,4 @@ Import ListNotations.
 
 Generalizable All Variables.
 
-(* Definition handler {ix} req : impure ix string := *)
-(*   let res := *)
-(*       match parse http_request req with *)
-(*       | inl _ => make_response client_error_BadRequest "" *)
-(*       | inr (Get uri) => *)
-(*         let resource := sandbox ([Dirname "opt"; Dirname "praecia"]) uri in *)
-(*         let path := uri_to_path resource in *)
-(*         var fd <- open path in *)
-(*         var content <- read fd in *)
-(*         close fd;; *)
-(*         make_response success_OK content *)
-(*       end *)
-(*   in pure (response_to_string res). *)
-
-Exec (http_server (ix := TCP <+> FILESYSTEM)).
+Exec http_server.
